1. The vector x can be found by subtracting the given vector from the vector on the right side of the equation. This can be done by subtracting each component of the vector on the right side from the corresponding component of the vector on the left side. x = (-2,-2,-2,6)

2. Find the vector C, if BC is three times shorter than AB.

A = (-1, 5, 1)
B = (2, 2, -2)

The vector C can be found by subtracting three times the vector BC from the vector AB.
The vector BC is calculated by subtracting the vector A from the vector B.
Vector BC = (2,2,-2) - (-1,5,1) = (3,-3,-3)
Vector C = (-1,5,1) - (3\*(3,-3,-3)) = (-10,24,10)
Therefore, the vector C is (-10,24,10).

3. No, the point (1, 2, 1) does not belong to the given line. To determine if a point belongs to a line, you need to check if the point lies on the line. To do this, you need to calculate the equation of the line using the two given vectors. The equation of the line is given by:
   V = V1 + t(V2 - V1) where t is a scalar.
   Substituting the given vectors into the equation, we get:
   V = (1, 1, 3) + t((2, 0, -1) - (1, 1, 3)) = (1, 1, 3) + t(-1, -1, -4)
   Solving for t, we get:
   t = (1 - 1)/(-1) = 0
   Substituting t = 0 into the equation, we get:
   V = (1, 1, 3) + 0((2, 0, -1) - (1, 1, 3)) = (1, 1, 3)
   Since (1, 2, 1) does not equal (1, 1, 3), the point (1, 2, 1) does not belong to the given line.

4. No, a vector set does not form a linear space unless it is closed under addition and scalar multiplication. This means that if you add two vectors in the set, the result must also be in the set, and if you multiply a vector in the set by a scalar, the result must also be in the set. Since the vector set you have described does not meet these criteria, it does not form a linear space.

- A + B in V
  (1,2) + (3,6) = (4,8)
  8 = 2 \* 4

- A + B = B + A
  (1,2) + (3,6) = (4,8)
  (3,6) = (1,2) = (4,8)
  8 = 2 \* 4

- (A + B) + C = A + (B + C)
  ((1,2) + (3,6)) + (7, 14) = (4,8) + (7,14) = (11,22)
  (1,2) + ((3,6) + (7, 14)) = (1,2) + (10, 20) = (11,22)
  22 = 2 \* 11

- A + 0 = A for all in V
  (1,2) + (0,0) = (1,2)
  2 = 2 \* 1

- A + -A = 0
  (1,2) + (-1 _ (1,2)) = (0,0)
  0 = 2 _ 0

- s _ A in V
  6 _ (3,6) = (18,36)
  36 = 2 \* 18

- (s1 + s2) _ A = s1 _ A + s2 _ A
  (4 + 3) _ (2,4)= 7 _ (2,4) = (14, 28)
  4 _ (2,4) + 3 _ (2,4) = (8,16) + (6, 12) = (14,28)
  28 = 2 _ 14

- s _ (A + B) = s _ A + s _ B
  3 _ ((1,2) + (5,10)) = 3 _ (6,12) = (18, 36)
  3 _ (1,2) + 3 _ (5,10) = (3,6) + (15,30) = (18, 36)
  36 = 2 _ 18

- (s1 _ s2) _ A = s1 _ (s2 _ A)
  (5 _ 2) _ (6, 12) = 10 _ (6,12) = (60, 120)
  5 _ (2 _ (6,12)) = 5 _ (12, 24) = (60, 120)
  120 = 2 \* 60

- 1 _ A = A
  1 _ (6, 12) = (6,12)
